Refactor soundness and completeness proofs

theories/Dynamics/Procedure.v
@@ -94,45 +94,27 @@ Instance relation_SqSubsetEq A B : SqSubsetEq (A → B → Prop) := refines A B.
 
 Definition monotone `{SqSubsetEq A, SqSubsetEq B} (f : A → B) := ∀ x y : A, x ⊑ y → f x ⊑ f y.
 
-Inductive snoc_list (A : Type) : Type :=
+(* Inductive list (A : Type) : Type :=
   | Nil
-  | Snoc (h : snoc_list A) (t : A).
+  | Snoc (h : list A) (t : A).
 
 Arguments Nil {_}.
 Arguments Snoc {_}.
 
-Notation "⟨⟩" := Nil (format "⟨⟩") : list_scope.
+Notation "[]" := Nil (format "[]") : list_scope.
 Notation "⟨ x ⟩" := (Snoc Nil x) : list_scope.
-Notation "⟨ x ; y ; .. ; z ⟩" := (Snoc .. (Snoc (Snoc Nil x) y) .. z) : list_scope.
+Notation "⟨ x ; y ; .. ; z ⟩" := (Snoc .. (Snoc (Snoc Nil x) y) .. z) : list_scope. *)
 
-Infix ",," := Snoc (at level 50, left associativity).
+Notation "l ,, x" := (x :: l) (at level 50, left associativity).
 
-Inductive SnocForall {A} (P : A → Prop) : snoc_list A → Prop :=
-  | SnocForall_nil : SnocForall P ⟨⟩
-  | SnocForall_cons x xs : SnocForall P xs → P x → SnocForall P (xs ,, x).
-
-Fixpoint snoc_list_of_list {A} (l : list A) :=
-  match l with
-  | [] => ⟨⟩
-  | h :: t => snoc_list_of_list t ,, h
-  end.
-
-Fixpoint SnocIn {A} (x : A) (l : snoc_list A) : Prop :=
-  match l with
-  | ⟨⟩ => False
-  | l ,, y => SnocIn x l ∨ x = y
-  end.
-
-Instance elem_of_snoc_list A : ElemOf A (snoc_list A) := SnocIn.
-
-Lemma not_in_neq {A} (x y : A) (xs : snoc_list A) : y ∉ xs ,, x → y ≠ x ∧ y ∉ xs.
+(* Lemma not_in_neq {A} (x y : A) (xs : list A) : y ∉ xs ,, x → y ≠ x ∧ y ∉ xs.
 Proof.
   unfold not. intros H. split.
   + intros Heq. apply H. cbn. now right.
   + intros Hin. apply H. cbn. now left.
 Qed.
 
-Lemma snoc_in_iff_list_in {A} (x : A) (l : list A) : x ∈ l ↔ x ∈ snoc_list_of_list l.
+Lemma snoc_in_iff_list_in {A} (x : A) (l : list A) : x ∈ l ↔ x ∈ list_of_list l.
 Proof.
   revert x. induction l.
   - intros x. split.
@@ -145,10 +127,10 @@ Proof.
     + intros [Hmem | Heq].
       * right. now apply IHl.
       * set_unfold. now left.
-Qed.
+Qed. *)
 
-Inductive δ_multi {Π Ω} `{EqDecision Π, Object Π Ω} {ω : Ω} : (type ω).(Σ) → (Π → status Π ω) → snoc_list Π → (type ω).(Σ) → (Π → status Π ω) → Prop :=
-  | δ_multi_refl σ f : δ_multi σ f ⟨⟩ σ f
+Inductive δ_multi {Π Ω} `{EqDecision Π, Object Π Ω} {ω : Ω} : (type ω).(Σ) → (Π → status Π ω) → list Π → (type ω).(Σ) → (Π → status Π ω) → Prop :=
+  | δ_multi_refl σ f : δ_multi σ f [] σ f
   | δ_multi_step f σ π πs op arg σ' res σ'' f' :
     δ_multi σ (f : Π → status Π ω) πs σ' (f' : Π → status Π ω) →
     (* if [π] has invoked [op(arg)], but not returned *)
@@ -157,23 +139,15 @@ Inductive δ_multi {Π Ω} `{EqDecision Π, Object Π Ω} {ω : Ω} : (type ω).
     (type ω).(δ) σ' π op arg σ'' res →
     δ_multi σ f (πs ,, π) σ'' (<[π := Linearized res]>f').
 
-Lemma δ_multi_mod `{EqDecision Π, Object Π Ω} {ω : Ω} (σ σ' : (type ω).(Σ)) (f f' : Π → status Π ω) (πs : snoc_list Π) (π : Π) (v : status Π ω) :
+Lemma δ_multi_mod `{EqDecision Π, Object Π Ω} {ω : Ω} (σ σ' : (type ω).(Σ)) (f f' : Π → status Π ω) (πs : list Π) (π : Π) (v : status Π ω) :
   π ∉ πs → δ_multi σ f πs σ' f' → δ_multi σ (<[π := v]>f) πs σ' (<[π := v]>f').
 Proof.
   revert σ' f'. induction πs.
   - intros σ' f' Hnotin Hstep. inv Hstep. constructor.
-  - intros σ' f' Hnotin Hstep. unfold not in Hnotin. apply not_in_neq in Hnotin as [Hneq Hnotin].
+  - intros σ' f' Hnotin Hstep. set_unfold in Hnotin. apply Decidable.not_or in Hnotin as [Hneq Hnotin].
     inv Hstep. rewrite Map.insert_comm at 1 by auto. econstructor; eauto.
     now rewrite Map.lookup_insert_ne at 1.
 Qed.
-
-(* Lemma δ_multi_trans {Π Ω} `{EqDecision Π, Object Π Ω} {ω : Ω} σ σ' σ'' (f f' f'' : Π → status Π ω) : 
-  δ_multi σ f σ' f' → δ_multi σ' f' σ'' f'' → δ_multi σ f σ'' f''.
-Proof.
-  intros Hmany Hmany'. generalize dependent Hmany. revert σ f. induction Hmany'.
-  - tauto.
-  - econstructor; eauto.
-Qed. *)
 
 Definition invoke `{EqDecision Π, Object Π Ω} {ω} (f : Π → status Π ω) (π : Π) (op : (type ω).(OP)) (arg : Value.t) : Π → status Π ω :=
   Map.insert π (Pending op arg) f.
@@ -187,22 +161,6 @@ Definition inhabited {A B} (R : A → B → Prop) : Prop := ∃ a b, R a b.
 
 Definition singleton {A B} (R : A → B → Prop) (x : A) (y : B) : Prop :=
   R x y ∧ ∀ x' y', R x' y' → x = x' ∧ y = y'.
-
-(* Variant evolve_inv `{EqDecision Π, Object Π Ω} {ω} (op : (type ω).(OP)) (π : Π) (arg : Value.t) (C : meta_configuration Π ω) : meta_configuration Π ω :=
-  evolve_inv_intro σ f πs σ' f' :
-    (* If (σ, f) ∈ C *)
-    C σ f →
-    f !!! π = Idle →
-    (* And atomic configuration (σ', f') results after linearizing every outstanding operation of [πs] *)
-    δ_multi σ (invoke f π op arg) πs σ' f' →
-    (* Then (σ', f') is in the resulting metaconfiguration *)
-    evolve_inv op π arg C σ' f'.
-
-Lemma evolve_inv_monotone `{EqDecision Π, Object Π Ω} {ω} (op : (type ω).(OP)) (π : Π) (arg : Value.t) : monotone (evolve_inv op π arg).
-Proof.
-  unfold monotone. intros x y Hless.
-  intros σ f Hevolve. inv Hevolve. econstructor; eauto.
-Qed. *)
 
 Variant map {A B C D} (f : A → B → (C * D)%type) (P : A → B → Prop) : C → D → Prop :=
   | map_intro a b c d :
@@ -328,9 +286,9 @@ Qed.
 
 Instance run_SubsetEq (C Π : Type) `{Object Π Ω} (ω : Ω) : SqSubsetEq (run C Π ω) := prefix C Π ω.
 
-Fixpoint behavior {C Π : Type} `{Object Π Ω} {ω : Ω} (r : run C Π ω) : snoc_list (Π * line Π ω) :=
+Fixpoint behavior {C Π : Type} `{Object Π Ω} {ω : Ω} (r : run C Π ω) : list (Π * line Π ω) :=
   match r with
-  | Initial _ => ⟨⟩
+  | Initial _ => []
   | Step r π l c =>
       match l with
       | Invoke _ _ | Response _ => behavior r ,, (π, l)
@@ -338,7 +296,7 @@ Fixpoint behavior {C Π : Type} `{Object Π Ω} {ω : Ω} (r : run C Π ω) : sn
       end
   end.
 
-Inductive subsequence {A : Type} : snoc_list A → snoc_list A → Prop :=
+Inductive subsequence {A : Type} : list A → list A → Prop :=
   | subsequence_refl l : subsequence l l
   | subsequence_trans l h t : subsequence l h → subsequence l (h ,, t).
 
@@ -467,25 +425,15 @@ Module Implementation.
   End Semantics.
 End Implementation.
 
-Module Augmented.
-
-  Section Auxillary.
-
-  Context {Aux : Type}.
-
-  Variable Σ : Aux → Type.
-
-  Variable σ₀ : Map.dependent Aux Σ.
+Module FullTracker.
 
   Record configuration Π Ω {Ω₀} `{Countable Π, Object Π Ω, Object Π Ω₀} (ω : Ω₀) := {
     base_configuration : Implementation.configuration Π Ω ω;
-    auxiliary_state : Map.dependent Aux Σ;
+    tracker : meta_configuration Π ω;
   }.
 
   Arguments base_configuration : default implicits.
-  Arguments auxiliary_state : default implicits.
-
-  Definition run Π Ω {Ω₀} `{Countable Π, Object Π Ω, Object Π Ω₀} (ω : Ω₀) := run (configuration Π Ω ω) Π ω.
+  Arguments tracker : default implicits.
 
   Section Semantics.
 
@@ -494,17 +442,19 @@ Module Augmented.
     Context `{Countable Π, Object Π Ω₀, Object Π Ω}.
 
     Variable impl : Implementation Π Ω ω.
+      
+    Variant initial_tracker : meta_configuration Π ω :=
+      initial_tracker_intro f : (∀ π, f !!! π = Idle) → initial_tracker impl.(initial_state) f.
 
-    Definition initial_configuration := {| auxiliary_state := σ₀; base_configuration := Implementation.initial_configuration impl |}.
-
-    (* Unlike normal objects, auxiliary objects can access other processes' local state *)
-    Variable step_auxiliary : Map.dependent Aux Σ → Π → line Π ω → Implementation.configuration Π Ω ω → Map.dependent Aux Σ → Prop.
+    Definition initial_configuration := {|
+      base_configuration := Implementation.initial_configuration impl;
+      tracker := initial_tracker;
+    |}.
 
     Variant step_augmented (c : configuration Π Ω ω) (π : Π) (l : line Π ω) : configuration Π Ω ω → Prop :=
-      | step_augmented_intro base f :
-        Implementation.step_configuration impl c.(base_configuration) π l base →
-          step_auxiliary c.(auxiliary_state) π l base f →
-            step_augmented c π l {| auxiliary_state := f; base_configuration := base |}.
+      | step_augmented_intro base :
+          Implementation.step_configuration impl c.(base_configuration) π l base →
+            step_augmented c π l {| tracker := evolve π l c.(tracker); base_configuration := base |}.
 
     Definition Run := Run initial_configuration step_augmented.
 
@@ -516,90 +466,84 @@ Module Augmented.
       | Step r π l c => Step (project r) π l c.(base_configuration)
       end.
 
-    (* Lemma project_sound r : Run r → Implementation.Run impl (project r).
+    Definition run := Procedure.run (configuration Π Ω ω) Π ω.
+
+    Fixpoint embed (r : Implementation.run Π Ω ω) : run :=
+      match r with
+      | Initial c => Initial {| base_configuration := c; tracker := initial_tracker |}
+      | Step r π l c =>
+        let r := embed r in
+        Step r π l ({| base_configuration := c; tracker := evolve π l (tracker (final r)) |})
+      end.
+
+  Inductive coupled : Implementation.run Π Ω ω → run → Prop :=
+    | coupled_initial c tracker : coupled (Initial c) (Initial {| tracker := tracker; base_configuration := c|})
+    | coupled_step r r' π l tracker base :
+      coupled r r' →
+      coupled
+        (Step r π l base)
+        (Step r' π l {| tracker := tracker; base_configuration := base |}).
+
+    Lemma project_embed_id r : project (embed r) = r.
     Proof.
-      induction r; intros.
-      - destruct c. simpl in *. econstructor. *)
+      induction r.
+      - reflexivity.
+      - cbn. congruence.
+    Qed.
 
-  End Semantics.
-  End Auxillary.
-End Augmented.
-
-Arguments Augmented.base_configuration : default implicits.
-Arguments Augmented.auxiliary_state : default implicits.
-
-(* Inductive coupled `{Countable Π, Object Π Ω, Object Π Ω₀} {ω : Ω₀} : Implementation.run Π Ω ω → Augmented.run Π Ω ω → Prop :=
-  | coupled_initial c tracker : coupled (Initial c) (Initial {| Augmented.tracker := tracker; Augmented.base_configuration := c|})
-  | coupled_step r r' π l tracker base :
-    coupled r r' →
-    coupled
-      (Step r π l base)
-      (Step r' π l {| Augmented.tracker := tracker; Augmented.base_configuration := base |}). *)
-
-(* relation (run (aumented_configuration Π Ω ω) Π ω) :=
-  | coupled_initial c : coupled (Initial c) (Initial c)
-  | coupled_step r r' π l tracker tracker' outstanding ϵ :
-    coupled r r' →
-    coupled
-      (Step r π l {| tracker := tracker; outstanding := outstanding; ϵ := ϵ |})
-      (Step r' π l {| tracker := tracker'; outstanding := outstanding; ϵ := ϵ |}). *)
-
-(* Variant linearization `{Countable Π, Object Π Ω₀, Object Π Ω} {ω : Ω₀} (impl : Implementation Π Ω ω) (r : run Π Ω ω) (atomic : run Π (sing ω) ω) : Prop :=
-  linearization_intro : 
-    Run impl r → Run (atomic_implementation ω impl.(initial_state)) atomic → behavior r = behavior atomic → linearization impl r atomic. *)
-
-
-Require Import Coq.Logic.Classical.
-
-Module PartialTracker.
-
-  Section Adequacy.
-
-  Context {Π Ω₀ Ω : Type} {ω : Ω₀}.
-
-  Context `{Countable Π, Object Π Ω₀, Object Π Ω}.
-
-  Variable impl : Implementation Π Ω ω.
-
-  Variant initial_tracker : meta_configuration Π ω :=
-    initial_tracker_intro f : (∀ π, f !!! π = Idle) → initial_tracker impl.(initial_state) f.
-
-  Section Soundness.
-
-    Context {Aux : Type}.
-
-    (* The metaconfiguration *)
-    Variable M : Aux.
-
-    Variable Σ : Aux → Type.
-
-    Variable σ₀ : Map.dependent Aux Σ.
-
-    (* The metaconfiguration has the appropriate type *)
-    Hypothesis M_meta_configuration : Σ M = meta_configuration Π ω.
-
-    Hint Rewrite M_meta_configuration : core.
-
-    Definition coerce : Σ M → meta_configuration Π ω.
+    Lemma embed_project_id r : Run r → embed (project r) = r.
     Proof.
-      rewrite M_meta_configuration. exact (λ x, x).
-    Defined.
+      induction r.
+      - intros Hrun. now inv Hrun.
+      - intros Hrun. inv Hrun. inv H7. cbn. f_equal.
+        + auto.
+        + f_equal. now rewrite IHr by auto.
+    Qed.
 
-    Variable step_auxiliary : 
-      Map.dependent Aux Σ → Π → line Π ω → Implementation.configuration Π Ω ω → Map.dependent Aux Σ → Prop.
+    Lemma project_coupled r : Run r → coupled (project r) r.
+    Proof.
+      induction r.
+      - intros Hrun. inv Hrun. constructor.
+      - intros Hrun. inv Hrun. inv H7. cbn. constructor. auto.
+    Qed.
 
-    Import Augmented.
+    Lemma project_wf r : Run r → Implementation.Run impl (project r).
+    Proof.
+      induction r.
+      - intros Hrun. inv Hrun. constructor.
+      - intros Hrun. inv Hrun. inv H7. cbn. constructor.
+        + now apply IHr.
+        + now destruct r.
+    Qed.
 
-    Definition run := run Σ Π Ω ω.
-  
-    Definition Run := Run Σ σ₀ impl step_auxiliary.
+    Lemma embed_wf r : Implementation.Run impl r → Run (embed r).
+    Proof.
+      induction r.
+      - intros Hrun. inv Hrun. constructor.
+      - intros Hrun. inv Hrun. cbn. constructor.
+        + now apply IHr.
+        + constructor. now destruct r.
+    Qed.
 
-    Definition tracker (r : run) := coerce ((final r).(auxiliary_state) M).
+    Lemma embed_behavior r : behavior (embed r) = behavior r.
+    Proof.
+      induction r.
+      - reflexivity.
+      - destruct l.
+        + cbn. now f_equal.
+        + auto.
+        + cbn. now f_equal.
+    Qed.
 
-    Variable refinement : 
-      ∀ r π l base f',
-        Run r →
-          step_auxiliary (final r).(auxiliary_state) π l base f' → coerce (f' M) ⊆ evolve π l (tracker r).
+    Lemma project_behavior r : behavior (project r) = behavior r.
+    Proof.
+      induction r.
+      - reflexivity.
+      - destruct l.
+        + cbn. f_equal. auto.
+        + auto.
+        + cbn. f_equal. auto.
+    Qed.
 
     Variant linearizable_run (r : run) σ f : Prop :=
       linearizable_intro (atomic : Atomic.run Π ω) :
@@ -608,14 +552,18 @@ Module PartialTracker.
             final atomic = (σ, f) →
               linearizable_run r σ f.
 
+    (* Lemma project_sound r : Run r → Implementation.Run impl (project r).
+    Proof.
+      induction r; intros.
+      - destruct c. simpl in *. econstructor. *)
     Definition tracker_sound (r : run) :=
-      ∀ σ f, tracker r σ f → linearizable_run r σ f.
+      ∀ σ f, tracker (final r) σ f → linearizable_run r σ f.
 
     Lemma sound_linearizations r atomic σ σ' πs f f' :
       Run r →
         Atomic.Run impl.(initial_state) atomic →
           behavior atomic = behavior r →
-            tracker r σ f →
+            tracker (final r) σ f →
               final atomic = (σ, f) →
                 δ_multi σ f πs σ' f' →
                   ∃ atomic',
@@ -638,21 +586,21 @@ Module PartialTracker.
       Run (Step r π (Invoke op arg) c) → tracker_sound r → tracker_sound (Step r π (Invoke op arg) c).
     Proof.
       intros HRunStep IH. inv HRunStep. inv H7. inv H2. unfold tracker_sound. simpl. intros.
-      eapply refinement in H2; eauto. inv H2. inv H5. remember (invoke f2 π op arg) in H6. induction H6.
+      inv H2. inv H3. remember (invoke f1 π op arg) in H5. induction H5.
       - intros. unfold tracker_sound in *.
         apply IH in H2. inversion H2.
         eapply linearizable_intro with (atomic := Step atomic π (Invoke op arg) _).
         + econstructor.
           * assumption.
-          * rewrite H8. now econstructor. 
-        + simpl. now rewrite H6. 
+          * rewrite H7. now econstructor. 
+        + simpl. now rewrite H5. 
         + simpl. now rewrite Heqs.
       - intros. unfold tracker_sound in *. simpl in *.
         apply IH in H2 as ?. inv H10. eapply IHδ_multi in H2. inv H2.
-        eapply linearizable_intro with (atomic := Step atomic0 π0 Intermediate _).
+        eapply linearizable_intro with (atomic := Step atomic π0 Intermediate _).
         + econstructor.
           * assumption.
-          * rewrite H17. simpl in *. econstructor; eauto.
+          * rewrite H14. simpl in *. econstructor; eauto.
         + assumption.
         + easy.
         + reflexivity.
@@ -662,16 +610,16 @@ Module PartialTracker.
       Run (Step r π Intermediate c) → tracker_sound r → tracker_sound (Step r π Intermediate c).
     Proof.
       intros HRunStep IH. inv HRunStep. inv H7. inv H2. unfold tracker_sound. simpl. intros.
-      eapply refinement in H2; eauto. inv H2. induction H8.
+      inv H2. induction H7.
       - intros. unfold tracker_sound in *.
-        apply IH in H7. inv H7.
+        apply IH in H6. inv H6.
         now eapply linearizable_intro with (atomic := atomic).
       - intros. unfold tracker_sound in *. simpl in *.
-        apply IH in H7 as ?. inv H11. eapply IHδ_multi in H7. inv H7.
+        apply IH in H6 as ?. inv H10. eapply IHδ_multi in H6. inv H6.
         eapply linearizable_intro with (atomic := Step atomic0 π0 Intermediate _).
         + econstructor.
           * assumption.
-          * rewrite H16. simpl in *. econstructor; eauto.
+          * rewrite H15. simpl in *. econstructor; eauto.
         + assumption.
         + reflexivity.
     Qed.
@@ -680,125 +628,264 @@ Module PartialTracker.
       Run (Step r π (Response v) c) → tracker_sound r → tracker_sound (Step r π (Response v) c).
     Proof.
       intros HRunStep IH. inv HRunStep. inv H7. inv H2. unfold tracker_sound. simpl. intros.
-      eapply refinement in H2; eauto. inv H2. inv H5. remember (ret f3 π) in H7. induction H7.
+      inv H2. inv H3. remember (ret f2 π) in H6. induction H6.
       - intros. unfold tracker_sound in *.
         apply IH in H2. inversion H2.
         eapply linearizable_intro with (atomic := Step atomic π (Response v) _).
         + econstructor.
           * assumption.
-          * rewrite H9. now econstructor. 
-        + simpl. now rewrite H7. 
+          * rewrite H8. now econstructor. 
+        + simpl. now rewrite H6. 
         + simpl. now rewrite Heqd.
       - intros. unfold tracker_sound in *. simpl in *.
-        apply IH in H2 as ?. inv H12. eapply IHδ_multi in H2; auto. inv H2.
+        apply IH in H2 as ?. inv H11. eapply IHδ_multi in H2; auto. inv H2.
         eapply linearizable_intro with (atomic := Step atomic0 π0 Intermediate _).
         + econstructor.
           * assumption.
-          * rewrite H17. simpl in *. econstructor; eauto.
+          * rewrite H16. simpl in *. econstructor; eauto.
         + assumption.
         + easy.
     Qed.
 
-  End Soundness.
+  Require Import Coq.Logic.FunctionalExtensionality.
 
-  Section StrongLinearizability.
+  Lemma sound r : Run r → tracker_sound r.
+  Proof.
+    induction r.
+    - simpl. intros. unfold tracker_sound. intros. econstructor.
+      + econstructor.
+      + constructor.
+      + inv H2. inv H3. cbn. f_equal. apply functional_extensionality. intros π. now change (f π) with (f !!! π).
+    - simpl. intros. inversion H2. destruct l.
+      + apply sound_invoke; auto.
+      + apply sound_intermediate; auto.
+      + apply sound_response; auto.
+  Qed.
 
-  Section Completeness.
+  Definition tracker_complete r := 
+    ∀ atomic σ f, 
+      Atomic.Run impl.(initial_state) atomic →
+        behavior r = behavior atomic →
+          final atomic = (σ, f) →
+            (final r).(tracker) σ f.
 
-    Definition unique {A B} (P : A → B → Prop) : Prop := ∀ a b b', P a b → P a b' → b = b'.
-
-    Definition linearization (r : Implementation.run Π Ω ω) (atomic : Atomic.run Π ω) := Atomic.Run impl.(initial_state) atomic ∧ behavior r = behavior atomic.
-
-    Hypothesis L : Implementation.run Π Ω ω → Atomic.configuration Π ω → Prop.
-
-    Hypothesis L_unique : unique L.
-
-    Hypothesis L_range : ∀ r, Implementation.Run impl r → ∃ conf, L r conf.
-
-    Hypothesis L_wf : ∀ r conf, L r conf → ∃ atomic, linearization r atomic ∧ final atomic = conf.
-
-    Variant Aux : Set := M | History.
-
-    Instance aux_eq_dec : EqDecision Aux.
-    Proof. solve_decision. Defined.
-
-    Definition Σ (aux : Aux) :=
-      match aux with
-      | M => meta_configuration Π ω
-      | History => Implementation.run Π Ω ω
-      end.
-
-    Variant step_auxiliary (aux : Map.dependent Aux Σ) (π : Π) (l : line Π ω) (base : Implementation.configuration Π Ω ω) : Map.dependent Aux Σ → Prop :=
-      step_auxiliary_intro :
-        step_auxiliary aux π l base 
-          (λ a,
-            let history := Step (aux History) π l base in
-            match a with
-            | M => λ σ f, L history (σ, f)
-            | History => history
-            end).
-
-    Definition σ₀ : Map.dependent Aux Σ.
+  Lemma linearization_invoke r π op arg c σ' f' atomic :
+    Atomic.Run impl.(initial_state) atomic →
+      behavior (Step r π (Invoke op arg) c) = behavior atomic →
+        (* If [atomic] is a linearization of run [r, (π, Invoke op arg), c] with final configuration [(σ', f')] *)
+        final atomic = (σ', f') →
+          Run (Step r π (Invoke op arg) c) →
+            ∃ atomic' σ f πs,
+              Atomic.Run impl.(initial_state) atomic' ∧
+                (* Then there exists some linearization [atomic'] of [r] *)
+                behavior r = behavior atomic' ∧
+                  (* With final configuration [(σ, f)] *)
+                  final atomic' = (σ, f) ∧
+                    (* Such that there exists some sequence of processes [πs] such 
+                      that (σ', f') results from first invoking [op(arg)] and then linearizing each of [πs] *)
+                    δ_multi σ (invoke f π op arg) πs σ' f' ∧
+                      f !!! π = Idle.
     Proof.
-      intros [ | ]; cbn.
-      - exact initial_tracker.
-      - exact (Initial (Implementation.initial_configuration impl)).
-    Defined.
+      intros Hatomic.
+      (* Need to generalize over the final configuration of the atomic run *)
+      revert σ' f'. 
+      (* Proceed by induction on the structure of the linearization *)
+      induction atomic.
+      - (* Case [atomic = Initial c']; impossible, as [atomic] is a linearization of [Step r π (Invoke op arg) c] *)
+        discriminate.
+      - (* Case [atomic = atomic, (π', l), c'] *)
+        intros.
+        (* Consider the last line [l] executed by the run *)
+        destruct l.
+        + (* [l] is an invocation *) 
+          simpl in *. 
+          (* Because the behavior of [atomic] is the same as [Step r π (Invoke op arg) c], this invocation must be [invoke π op arg] *)
+          inv H2.
+          (* We can take [atomic] as the linearization of [r] *)
+          exists atomic.
+          destruct (final atomic) as [σ f] eqn:Hfinal. exists σ. exists f.
+          (* Because the last step of the linearization is an invocation, no pending processes linearize afterwards *)
+          exists [].
+          split.
+          * (* Because [atomic, (π', l), c'] is an atomic run, so is [atomic] *)
+            inv Hatomic. assumption.
+          * split.
+            -- assumption.
+            -- split.
+              ++ reflexivity.
+              ++ inv Hatomic. inv H8. unfold invoke.
+                  assert ((σ', f0) = (σ, f)) by now transitivity (final atomic).
+                  inv H3. split.
+                ** constructor.
+                ** assumption.
+        + (* [l] is an intermediate line, so [atomic, (π', l), c'] is also a linearization of [Step r π (Invoke op arg) c] *) 
+          simpl in *.
+          (* Because [atomic, (π', l), c'] is an atomic run, so is [atomic] *)
+          inv Hatomic. subst.
+          (* Let (σ, f) be the final configuration of [atomic ]
+            Because ((σ, f), (π', Intermediate), (σ', f')) is a step,
+            [f π' = Pending op' arg'], and [(σ', f')] results from linearizing [op(arg)] *)
+          inv H10.
+          apply IHatomic with (σ' := σ) (f' := f) in H7 as ?; eauto.
+          (* We can apply the induction hypothesis to [atomic] *)
+          destruct H5 as [atomic' [σ'' [f'' [πs [? [? [? [? ?]]]]]]]].
+          exists atomic'. exists σ''. exists f''.
+          exists (πs ,, π0).
+          split.
+          * assumption.
+          * split.
+            -- assumption.
+            -- split.
+              ** assumption.
+              ** split.
+                --- econstructor; eauto.
+                --- assumption.
+        + discriminate.
+  Qed.
 
-    (* Check Augmented.invariant Σ σ₀ impl step_auxiliary (λ _, True). *)
-
-    Import Augmented.
-
-    Lemma completeness :
-      ∀ r π l base f',
-        Run Σ σ₀ impl step_auxiliary r →
-          step_auxiliary (final r).(auxiliary_state) π l base f' → f' M ⊆ evolve π l ((final r).(auxiliary_state) M).
+  Lemma linearization_response r π v c σ' f' atomic :
+    Atomic.Run impl.(initial_state) atomic →
+      behavior (Step r π (Response v) c) = behavior atomic →
+        (* If [atomic] is a linearization of run [r, (π, Response v), c] with final configuration [(σ', f')] *)
+        final atomic = (σ', f') →
+          Run (Step r π (Response v) c) →
+            ∃ atomic' σ f πs,
+              Atomic.Run impl.(initial_state) atomic' ∧
+                (* Then there exists some linearization [atomic'] of [r] *)
+                behavior r = behavior atomic' ∧
+                  (* With final configuration [(σ, f)] *)
+                  final atomic' = (σ, f) ∧
+                    (* Such that there exists some sequence of processes [πs] such 
+                      that (σ', f') results from first invoking [op(arg)] and then linearizing each of [πs] *)
+                    δ_multi σ (ret f π) πs σ' f' ∧
+                      f !!! π = Linearized v.
     Proof.
-      induction r eqn:?.
-      (* Is actually trivial, does not require induction *)
-    Admitted.
-    
-    End Completeness.
-  
-    End StrongLinearizability.
+      intros Hatomic.
+      (* Need to generalize over the final configuration of the atomic run *)
+      revert σ' f'. 
+      (* Proceed by induction on the structure of the linearization *)
+      induction atomic.
+      - (* Case [atomic = Initial c']; impossible, as [atomic] is a linearization of [Step r π (Invoke op arg) c] *)
+        discriminate.
+      - (* Case [atomic = atomic, (π', l), c'] *)
+        intros.
+        (* Consider the last line [l] executed by the run *)
+        destruct l.
+        + discriminate.
+        + (* [l] is an intermediate line, so [atomic, (π', l), c'] is also a linearization of [Step r π (Invoke op arg) c] *) 
+          simpl in *.
+          (* Because [atomic, (π', l), c'] is an atomic run, so is [atomic] *)
+          inv Hatomic. subst.
+          (* Let (σ, f) be the final configuration of [atomic ]
+            Because ((σ, f), (π', Intermediate), (σ', f')) is a step,
+            [f π' = Pending op' arg'], and [(σ', f')] results from linearizing [op(arg)] *)
+          inv H10.
+          apply IHatomic with (σ' := σ) (f' := f) in H7 as ?; eauto.
+          (* We can apply the induction hypothesis to [atomic] *)
+          destruct H5 as [atomic' [σ'' [f'' [πs [? [? [? [? ?]]]]]]]].
+          exists atomic'. exists σ''. exists f''.
+          exists (πs ,, π0).
+          split.
+          * assumption.
+          * split.
+            -- assumption.
+            -- split.
+              ** assumption.
+              ** split.
+                --- econstructor; eauto.
+                --- assumption.
+        + (* [l] is a response *) 
+          simpl in *. 
+          (* Because the behavior of [atomic] is the same as [Step r π (Response v) c], this response must be [Response v] *)
+          inv H2.
+          (* We can take [atomic] as the linearization of [r] *)
+          exists atomic.
+          destruct (final atomic) as [σ f] eqn:Hfinal. exists σ. exists f.
+          (* Because the last step of the linearization is an invocation, no pending processes linearize afterwards *)
+          exists [].
+          split.
+          * (* Because [atomic, (π', l), c'] is an atomic run, so is [atomic] *)
+            inv Hatomic. assumption.
+          * split.
+            -- assumption.
+            -- split.
+              ++ reflexivity.
+              ++ inv Hatomic. inv H9. unfold invoke.
+                assert ((σ', f0) = (σ, f)) by now transitivity (final atomic).
+                inv H3. split.
+                ** constructor.
+                ** assumption.
+  Qed.
 
-End Adequacy.
+  (* Every linearization of an initial run is also initial *)
+  Lemma linearization_empty c atomic :
+    Run (Initial c) → Atomic.Run impl.(initial_state) atomic → behavior (Initial c) = behavior atomic → atomic = Initial (impl.(initial_state), λ _, Idle).
+  Proof.
+    simpl. intros Hrun. inv Hrun. induction atomic.
+    - intros. inv H2. reflexivity.
+    - intros. inv H2. destruct l; simpl in *.
+      + discriminate.
+      + apply IHatomic in H6; auto. inv H9. simpl in *. inv H2.
+      + discriminate.
+  Qed.
 
-End PartialTracker.
+  Lemma complete r atomic σ f : Run r → Atomic.Run impl.(initial_state) atomic → behavior r = behavior atomic → final atomic = (σ, f) → (final r).(tracker) σ f.
+  Proof.
+    revert atomic σ f.
+    induction r.
+    - simpl. intros. eapply linearization_empty in H2 as ?; eauto. 
+      subst. simpl in *. inv H5. inv H2. simpl. now econstructor.
+    - destruct l.
+      + intros. cbn. eapply linearization_invoke in H3 as (atomic' & σ' & f' & πs & Hatomicrun & Hbeh & Hfinal & Hmulti & Hidle); eauto.
+        simpl in *. inv H2. inv H10. inv H2. simpl. econstructor.
+        * econstructor; eauto.
+        * eassumption.
+      + simpl in *. intros. inv H2. inv H11. simpl. econstructor.
+        * eapply IHr; eauto.
+        * econstructor.
+      + intros. eapply linearization_response in H3 as (atomic' & σ' & f' & πs & Hatomicrun & Hbeh & Hfinal & Hmulti & Hidle); eauto.
+        simpl in *. inv H2. inv H10. simpl. econstructor.
+        * econstructor; eauto. 
+        * eauto.
+  Qed.
 
-Module FullTracker.
+  (** An implementation is linearizable iff there exists a linearization for each of its runs *)
+  Definition linearizable :=
+    ∀ r,
+      Implementation.Run impl r →
+        ∃ atomic, Atomic.Run impl.(initial_state) atomic ∧ behavior r = behavior atomic.
 
-  Definition Aux : Type := ().
+  Lemma soundness : invariant (λ c, ∃ σ f, tracker c σ f) → linearizable.
+  Proof.
+    unfold linearizable, invariant. intros Hinv r Hrun.
+    pose proof Hinv (embed r) (embed_wf r Hrun) as (σ & f & Hmeta).
+    pose proof sound (embed r) (embed_wf r Hrun).
+    unfold tracker_sound in *.
+    pose proof H2 _ _ Hmeta as [atomic Hatomic Hlinearization Hfinal].
+    exists atomic. split.
+    - assumption.
+    - rewrite <- Hlinearization. now rewrite embed_behavior. 
+  Qed.
 
-  Definition Σ Π `{Object Π Ω} (ω : Ω) : Aux → Type := const (meta_configuration Π ω).
+  Lemma completeness : linearizable → invariant (λ c, ∃ σ f, tracker c σ f).
+  Proof.
+    unfold linearizable, invariant. intros Hlinearizable r Hrun.
+    pose proof Hlinearizable (project r) (project_wf r Hrun) as (atomic & Hatomic & Hbehavior).
+    destruct (final atomic) as [σ f] eqn:Hfinal.
+    exists σ. exists f.
+    eapply complete; eauto.
+    rewrite <- Hbehavior. now rewrite project_behavior.
+  Qed.
 
-  Definition run Π Ω `{Countable Π, Object Π Ω, Object Π Ω₀} (ω : Ω₀) := Augmented.run (Σ Π ω) Π Ω ω.
+  (* An implementation is linearizable iff its tracker being non-empty is an invariant of the algorithm *)
+  Theorem adequacy : linearizable ↔ invariant (λ c, ∃ σ f, tracker c σ f).
+  Proof.
+    split.
+    - exact completeness.
+    - exact soundness.
+  Qed.
 
-  Definition configuration Π Ω `{Countable Π, Object Π Ω, Object Π Ω₀} (ω : Ω₀) := Augmented.configuration (Σ Π ω) Π Ω ω.
-
-  Section Adequacy.
-
-  Context {Π Ω₀ Ω : Type} {ω : Ω₀}.
-
-  Context `{Countable Π, Object Π Ω₀, Object Π Ω}.
-
-  Variable impl : Implementation Π Ω ω.
-
-  Definition initial_tracker := PartialTracker.initial_tracker impl.
-
-  Definition σ₀ : Map.dependent Aux (Σ Π ω) := const initial_tracker.
-
-  Variant step_auxiliary (C : Map.dependent Aux (Σ Π ω)) (π : Π) (l : line Π ω) (c : Implementation.configuration Π Ω ω) : Map.dependent Aux (Σ Π ω) → Prop :=
-    | step_auxiliary_intro : step_auxiliary C π l c (const (evolve π l (C tt))).
-
-  Definition Run := Augmented.Run (Σ Π ω) σ₀ impl step_auxiliary.
-
-  Definition tracker (c : configuration Π Ω ω) := c.(Augmented.auxiliary_state) tt.
-
-  Definition invariant p := Augmented.invariant (Σ Π ω) σ₀ impl step_auxiliary (λ c, p c.(Augmented.base_configuration) (c.(Augmented.auxiliary_state) tt)).
-
-  End Adequacy.
-
+  End Semantics.
 End FullTracker.
 
 Module ReadWrite.
@@ -884,7 +971,6 @@ Section RWCAS.
     (* Only auxiliary state is metaconfiguration *)
     Definition Aux := unit.
 
-    Import Augmented.
     Import Implementation.
 
     Variant tracker_inv (c : Implementation.configuration Π ReadCAS.t ReadWrite.Cell) (π : Π) : status Π ReadWrite.Cell → Type :=
@@ -1365,7 +1451,7 @@ Section RWCAS.
       Lemma linearized_writers_correct {base f} (X : ∀ π : Π, tracker_inv base π (f !!! π)) (l : gset Π) :
         (∀ π : Π, π ∈ l ↔ f !!! π ≠ Idle) →
           ∀ π,
-            π ∈ snoc_list_of_list (linearized_writers X (elements l)) ↔ linearized_writer X π.
+            π ∈ list_of_list (linearized_writers X (elements l)) ↔ linearized_writer X π.
       Proof.
         intros Hmem π. unfold linearized_writers. rewrite <- snoc_in_iff_list_in. rewrite elem_of_list_In.
         rewrite filter_In. split.
@@ -1375,9 +1461,9 @@ Section RWCAS.
           + reflexivity.
       Qed.
 
-      Fixpoint linearize_many (πs : snoc_list Π) (f : Π → status Π ReadWrite.Cell) :=
+      Fixpoint linearize_many (πs : list Π) (f : Π → status Π ReadWrite.Cell) :=
         match πs with
-        | ⟨⟩ => f
+        | [] => f
         | πs ,, π => <[π := Linearized Value.Unit]>(linearize_many πs f)
         end.
 
@@ -1439,7 +1525,7 @@ Section RWCAS.
 
       Lemma linearize_writers_step {base f} (X : ∀ π : Π, tracker_inv base π (f !!! π)) (l : gset Π) σ :
         (∀ π : Π, π ∈ l ↔ f !!! π ≠ Idle) →
-          ∃ σ', δ_multi σ (update X) (snoc_list_of_list (linearized_writers X (elements l))) σ' f.
+          ∃ σ', δ_multi σ (update X) (list_of_list (linearized_writers X (elements l))) σ' f.
       Proof.
         intros Hout. pose proof linearized_writers_correct X l Hout as Hlin. clear Hout.
         generalize dependent X. revert f. assert (NoDup (elements l)) as Hunique by apply NoDup_elements. induction (elements l).
@@ -1550,7 +1636,7 @@ Section RWCAS.
             { unfold invoke, insert, Map.map_insert.
               rewrite H1. unfold "!!!", Map.map_lookup_total.
               now rewrite Map.Dep.insert_insert. }
-            eapply linearize_pending_intro with (πs := ⟨⟩) (f := g) (σ := ϵ base Cell).
+            eapply linearize_pending_intro with (πs := []) (f := g) (σ := ϵ base Cell).
             -- rewrite H4. econstructor.
               ++ apply IHr.
                 ** auto.
@@ -1576,7 +1662,7 @@ Section RWCAS.
                 eapply linearize_pending_intro 
                   with
                   (f := <[π := @Pending Π ReadWrite.t _ _ ReadWrite.Cell _ arg0]> g)
-                  (πs := ⟨⟩ ,, π)
+                  (πs := [] ,, π)
                   (σ := ϵ base Cell).
                 instantiate (1 := ReadWrite.Read).
               ** eapply IHr; eauto. rewrite <- H6. econstructor.
@@ -1630,7 +1716,7 @@ Section RWCAS.
                  rewrite <- Map.insert_insert with (k := π) (v := Pending f.(op) f.(arg)).
                  apply linearize_pending_intro
                   with 
-                    (πs := snoc_list_of_list (linearized_writers X (elements l)) ,, π)
+                    (πs := list_of_list (linearized_writers X (elements l)) ,, π)
                     (f := <[π := Pending f.(op) f.(arg)]>(update X))
                     (σ := ϵ (base_configuration (final r)) Cell).
                 ** eapply IHr; eauto. econstructor.
@@ -1663,7 +1749,7 @@ Section RWCAS.
                     --- subst. cbn. fold (Map.lookup Cell (Map.insert Cell σ (ϵ (base_configuration (final r))))).
                         rewrite Map.Dep.lookup_insert. constructor.          
               ++ rewrite Map.Dep.η in H6 by assumption.
-                 apply linearize_pending_intro with  (πs := ⟨⟩) (f := g) (σ := ϵ base Cell).
+                 apply linearize_pending_intro with  (πs := []) (f := g) (σ := ϵ base Cell).
                  ** auto. apply IHr; auto. rewrite <- H6. econstructor. intros π'.
                     destruct (decide (π = π')).
                     --- subst. rewrite <- H1. eapply tracker_inv_write_cas_linearized; eauto.
@@ -1678,7 +1764,7 @@ Section RWCAS.
             assert (g = ret (<[π := Linearized v]> g) π).
             { unfold ret. rewrite H1. unfold insert, Map.map_insert, lookup_total, Map.map_lookup_total.
               now rewrite Map.Dep.insert_insert. }
-            apply linearize_pending_intro with (πs := ⟨⟩) (f := g) (σ := ϵ base Cell).
+            apply linearize_pending_intro with (πs := []) (f := g) (σ := ϵ base Cell).
             -- rewrite H0. econstructor.
               ++ apply IHr.
                 ** assumption.
@@ -1704,736 +1790,3 @@ Section RWCAS.
       Qed.
 
 End RWCAS.
-
-Module FullTracker (Impl : Implementation).
-  
-  Module Sem <: Semantics.
-
-    Include Impl.
-
-    Variant step `{Countable Π, Object Π Ω₀, Object Π Ω} (C : meta_configuration Π ω) (π : Π) (l : line Π ω) : meta_configuration Π ω → Prop :=
-      Aacker : step C π l (evolve π l C).
-
-    Definition step_tracker `{Countable Π, Object Π Ω₀, Object Π Ω} := step.
-
-  End Sem.
-
-  Include Augmented Sem.
-
-End FullTracker.
-
-
-Module Adequacy (Impl : Implementation).
-
-  Module Full := FullTracker Impl.
-  Module Partial := PartialTracker Impl.
-
-  Include Impl.
-
-  Context `{Countable Π, Object Π Ω₀, Object Π Ω}.
-
-  Variant linearizable_run (r : run (configuration Π Ω ω) Π ω) σ f : Prop :=
-    linearizable_intro atomic :
-      Atomic.Run impl.(initial_state) atomic →
-        behavior r = behavior atomic →
-          final atomic = (σ, f) →
-            linearizable_run r σ f.
-
-  Definition tracker_sound (r : run (configuration Π Ω ω) Π ω) :=
-    ∀ σ f, (final r).(tracker) σ f → linearizable_run r σ f.
-
-  Lemma sound_linearizations r atomic σ σ' πs f f' :
-    Full.Run r →
-      Atomic.Run impl.(initial_state) atomic →
-        behavior atomic = behavior r →
-          (final r).(tracker) σ f →
-            final atomic = (σ, f) →
-              δ_multi σ f πs σ' f' →
-                ∃ atomic',
-                  Atomic.Run impl.(initial_state) atomic' ∧
-                    behavior atomic' = behavior r ∧
-                      final atomic' = (σ', f').
-  Proof.
-    revert σ' f'. induction πs.
-    - intros. exists atomic. split.
-      + assumption.
-      + now inv H7.
-    - intros. inv H7. pose proof IHπs σ'0 f'0 as IH. eapply IH in H2; eauto.
-      destruct H2 as (atomic' & Hatomic & Hbehavior & Hfinal).
-      eexists (Step atomic' t Intermediate _).
-      split.
-      + econstructor; eauto. rewrite Hfinal. econstructor; eauto.
-      + now split.
-  Qed.
-
-  Lemma sound_invoke r π op arg c :
-    Full.Run (Step r π (Invoke op arg) c) → tracker_sound r → tracker_sound (Step r π (Invoke op arg) c).
-  Proof.
-    intros HRunStep IH. inv HRunStep. inv H7. inv H3.  unfold tracker_sound. simpl. intros.
-    rewrite <- H6 in H3. inv H3. generalize dependent f. generalize dependent σ. induction πs.
-    - intros. unfold tracker_sound in *. inv H13.
-      apply IH in H8. inv H8.
-      eapply linearizable_intro with (atomic := Step atomic π (Invoke op arg) _).
-      + econstructor.
-        * assumption.
-        * rewrite H7. now econstructor. 
-      + simpl. now rewrite H5. 
-      + reflexivity.
-    - intros. inv H13. unfold tracker_sound in *. simpl in *.
-      apply IH in H8. inv H8. eapply IHπs in H7. inv H7.
-      eapply linearizable_intro with (atomic := Step atomic0 t Intermediate _).
-      + econstructor.
-        * assumption.
-        * rewrite H13. simpl in *. econstructor; eauto.
-      + assumption.
-      + easy.
-  Qed.
-
-  Lemma step_intermediate_idempotent :
-
-
-  Lemma sound_intermediate r π c :
-    Full.Run (Step r π Intermediate c) → tracker_sound r → tracker_sound (Step r π Intermediate c).
-  Proof.
-
-
-  Lemma sound_intermediate r π c :
-    Full.Run (Step r π Intermediate c) → tracker_sound r → tracker_sound (Step r π Intermediate c).
-  Proof.
-    intros HRunStep IH. inv HRunStep. inv H7. unfold tracker_sound. simpl. intros. inv H3.
-    rewrite <- H7 in H5. inv H5. generalize dependent f0. generalize dependent σ. induction πs.
-    - intros. unfold tracker_sound in *. simpl in *. inv H6.
-      apply IH in H3. inv H3. 
-      now apply linearizable_intro with (atomic := atomic).
-    - intros. inv H6. unfold tracker_sound in *.
-      apply IH in H3 as ?. inv H5. eapply IHπs in H3.
-      + admit.
-      + 
-      inv H3.
-      eapply linearizable_intro with (atomic := Step atomic0 t Intermediate _).
-      + econstructor.
-        * assumption.
-        * rewrite H13. simpl in *. econstructor; eauto.
-      + assumption.
-      + easy.
-  Qed.
-
-  Lemma sound_response r π v c :
-    Implementation.Run impl (Step r π (Response v) c) → tracker_sound r → tracker_sound (Step r π (Response v) c).
-  Proof.
-    intros HRunStep IH. inv HRunStep. inv H7. unfold tracker_sound. simpl. intros. inv H3.
-    generalize dependent f0. generalize dependent σ. induction πs.
-    - intros. unfold tracker_sound in *. rewrite <- H2 in IH. simpl in *. inv H9.
-      apply IH in H7. inv H7.
-      eapply linearizable_intro with (atomic := Step atomic π (Response v) _).
-      + econstructor.
-        * assumption.
-        * rewrite H10. now econstructor. 
-      + simpl. now rewrite H9. 
-      + reflexivity.
-    - intros. inv H9. unfold tracker_sound in *. rewrite <- H2 in IH. simpl in *.
-      apply IH in H7. inv H5. eapply IHπs in H11. inv H11.
-      eapply linearizable_intro with (atomic := Step atomic t Intermediate _).
-      + econstructor.
-        * assumption.
-        * rewrite H10. simpl in *. econstructor; eauto.
-      + assumption.
-      + easy.
-  Qed.
-
-  (* Lemma sound r σ f :
-    FullTracker.Run impl r →
-      (final r).(tracker) σ f →
-        ∃ atomic,
-          Atomic.Run impl.(initial_state) atomic ∧ behavior atomic = behavior r ∧ final atomic = (σ, f).
-  Proof.
-    revert σ f. induction r.
-    - simpl. intros σ f Hrun Htracker. eexists (Initial _). split.
-      + econstructor.
-      + split.
-        * reflexivity.
-        * inv Hrun. simpl in *. now inv Htracker. 
-    - intros. simpl in *. inversion H2. subst.
-      inv H9. inv H5. pose proof H3 as Htracker. rewrite <- H8 in H3. inv H3.
-      + eapply IHr in H6 as (atomic & Hatomic & Hbehavior & Hfinal); eauto.
-        eapply sound_linearizations with (atomic := Step atomic π (Invoke op arg) _) in H2.
-        * shelve.
-        * econstructor; eauto. rewrite Hfinal. now econstructor.
-        * simpl. now rewrite Hbehavior.
-        * simpl. rewrite <- H8. econstructor.
-          -- eassumption.
-          -- assumption.
-          -- econstructor.
-        * reflexivity.
-        * eassumption.
-        Unshelve. simpl in *.
-        inv H2 as (atomic' & ? & ? & ?). exists atomic'. split.
-        -- assumption.
-        -- now split.
-      + eapply IHr in H6 as (atomic & Hatomic & Hbehavior & Hfinal).
-        eapply sound_linearizations with (atomic := Step atomic π (Invoke op arg) _) in H2.
-        * shelve.
-        * econstructor; eauto. rewrite Hfinal. now econstructor.
-        * simpl. now rewrite Hbehavior.
-        * simpl. rewrite <- H8. econstructor.
-          -- eassumption.
-          -- assumption.
-          -- econstructor.
-        * reflexivity.
-        * eassumption.
-        Unshelve. simpl in *.
-        inv H2 as (atomic' & ? & ? & ?). exists atomic'. split.
-        -- assumption.
-        -- now split.
-        
-
-
-      apply sound_invoke; auto.
-      + apply sound_intermediate; auto.
-      + apply sound_response; auto.
-  Qed. *)
-
-  Definition tracker_complete r := 
-    ∀ atomic σ f, 
-      Atomic.Run impl.(initial_state) atomic →
-        behavior r = behavior atomic →
-          final atomic = (σ, f) →
-            (final r).(tracker) σ f.
-
-  Lemma linearization_invoke r π op arg c σ' f' atomic :
-    Atomic.Run impl.(initial_state) atomic →
-      behavior (Step r π (Invoke op arg) c) = behavior atomic →
-        (* If [atomic] is a linearization of run [r, (π, Invoke op arg), c] with final configuration [(σ', f')] *)
-        final atomic = (σ', f') →
-          Implementation.Run impl (Step r π (Invoke op arg) c) →
-            ∃ atomic' σ f πs,
-              Atomic.Run impl.(initial_state) atomic' ∧
-                (* Then there exists some linearization [atomic'] of [r] *)
-                behavior r = behavior atomic' ∧
-                  (* With final configuration [(σ, f)] *)
-                  final atomic' = (σ, f) ∧
-                    (* Such that there exists some sequence of processes [πs] such 
-                      that (σ', f') results from first invoking [op(arg)] and then linearizing each of [πs] *)
-                    δ_multi σ (invoke f π op arg) πs σ' f' ∧
-                      f !!! π = Idle.
-    Proof.
-      intros Hatomic.
-      (* Need to generalize over the final configuration of the atomic run *)
-      revert σ' f'. 
-      (* Proceed by induction on the structure of the linearization *)
-      induction atomic.
-      - (* Case [atomic = Initial c']; impossible, as [atomic] is a linearization of [Step r π (Invoke op arg) c] *)
-        discriminate.
-      - (* Case [atomic = atomic, (π', l), c'] *)
-        intros.
-        (* Consider the last line [l] executed by the run *)
-        destruct l.
-        + (* [l] is an invocation *) 
-          simpl in *. 
-          (* Because the behavior of [atomic] is the same as [Step r π (Invoke op arg) c], this invocation must be [invoke π op arg] *)
-          inv H2.
-          (* We can take [atomic] as the linearization of [r] *)
-          exists atomic.
-          destruct (final atomic) as [σ f] eqn:Hfinal. exists σ. exists f.
-          (* Because the last step of the linearization is an invocation, no pending processes linearize afterwards *)
-          exists ⟨⟩.
-          split.
-          * (* Because [atomic, (π', l), c'] is an atomic run, so is [atomic] *)
-            inv Hatomic. assumption.
-          * split.
-            -- assumption.
-            -- split.
-              ++ reflexivity.
-              ++ inv Hatomic. inv H9. unfold invoke.
-                  assert ((σ', f0) = (σ, f)) by now transitivity (final atomic).
-                  inv H3. split.
-                ** constructor.
-                ** assumption.
-        + (* [l] is an intermediate line, so [atomic, (π', l), c'] is also a linearization of [Step r π (Invoke op arg) c] *) 
-          simpl in *.
-          (* Because [atomic, (π', l), c'] is an atomic run, so is [atomic] *)
-          inv Hatomic. subst.
-          (* Let (σ, f) be the final configuration of [atomic ]
-            Because ((σ, f), (π', Intermediate), (σ', f')) is a step,
-            [f π' = Pending op' arg'], and [(σ', f')] results from linearizing [op(arg)] *)
-          inv H10.
-          apply IHatomic with (σ' := σ) (f' := f) in H7 as ?; eauto.
-          (* We can apply the induction hypothesis to [atomic] *)
-          destruct H5 as [atomic' [σ'' [f'' [πs [? [? [? [? ?]]]]]]]].
-          exists atomic'. exists σ''. exists f''.
-          exists (πs ,, π0).
-          split.
-          * assumption.
-          * split.
-            -- assumption.
-            -- split.
-              ** assumption.
-              ** split.
-                --- econstructor; eauto.
-                --- assumption.
-        + discriminate.
-  Qed.
-
-  Lemma linearization_response r π v c σ' f' atomic :
-    Atomic.Run impl.(initial_state) atomic →
-      behavior (Step r π (Response v) c) = behavior atomic →
-        (* If [atomic] is a linearization of run [r, (π, Response v), c] with final configuration [(σ', f')] *)
-        final atomic = (σ', f') →
-          Implementation.Run impl (Step r π (Response v) c) →
-            ∃ atomic' σ f πs,
-              Atomic.Run impl.(initial_state) atomic' ∧
-                (* Then there exists some linearization [atomic'] of [r] *)
-                behavior r = behavior atomic' ∧
-                  (* With final configuration [(σ, f)] *)
-                  final atomic' = (σ, f) ∧
-                    (* Such that there exists some sequence of processes [πs] such 
-                      that (σ', f') results from first invoking [op(arg)] and then linearizing each of [πs] *)
-                    δ_multi σ (ret f π) πs σ' f' ∧
-                      f !!! π = Linearized v.
-    Proof.
-      intros Hatomic.
-      (* Need to generalize over the final configuration of the atomic run *)
-      revert σ' f'. 
-      (* Proceed by induction on the structure of the linearization *)
-      induction atomic.
-      - (* Case [atomic = Initial c']; impossible, as [atomic] is a linearization of [Step r π (Invoke op arg) c] *)
-        discriminate.
-      - (* Case [atomic = atomic, (π', l), c'] *)
-        intros.
-        (* Consider the last line [l] executed by the run *)
-        destruct l.
-        + discriminate.
-        + (* [l] is an intermediate line, so [atomic, (π', l), c'] is also a linearization of [Step r π (Invoke op arg) c] *) 
-          simpl in *.
-          (* Because [atomic, (π', l), c'] is an atomic run, so is [atomic] *)
-          inv Hatomic. subst.
-          (* Let (σ, f) be the final configuration of [atomic ]
-            Because ((σ, f), (π', Intermediate), (σ', f')) is a step,
-            [f π' = Pending op' arg'], and [(σ', f')] results from linearizing [op(arg)] *)
-          inv H10.
-          apply IHatomic with (σ' := σ) (f' := f) in H7 as ?; eauto.
-          (* We can apply the induction hypothesis to [atomic] *)
-          destruct H5 as [atomic' [σ'' [f'' [πs [? [? [? [? ?]]]]]]]].
-          exists atomic'. exists σ''. exists f''.
-          exists (πs ,, π0).
-          split.
-          * assumption.
-          * split.
-            -- assumption.
-            -- split.
-              ** assumption.
-              ** split.
-                --- econstructor; eauto.
-                --- assumption.
-        + (* [l] is a response *) 
-          simpl in *. 
-          (* Because the behavior of [atomic] is the same as [Step r π (Response v) c], this response must be [Response v] *)
-          inv H2.
-          (* We can take [atomic] as the linearization of [r] *)
-          exists atomic.
-          destruct (final atomic) as [σ f] eqn:Hfinal. exists σ. exists f.
-          (* Because the last step of the linearization is an invocation, no pending processes linearize afterwards *)
-          exists ⟨⟩.
-          split.
-          * (* Because [atomic, (π', l), c'] is an atomic run, so is [atomic] *)
-            inv Hatomic. assumption.
-          * split.
-            -- assumption.
-            -- split.
-              ++ reflexivity.
-              ++ inv Hatomic. inv H9. unfold invoke.
-                assert ((σ', f0) = (σ, f)) by now transitivity (final atomic).
-                inv H3. split.
-                ** constructor.
-                ** assumption.
-  Qed.
-
-  (* Every linearization of an initial run is also initial *)
-  Lemma linearization_empty c atomic :
-    Implementation.Run impl (Initial c) → Atomic.Run impl.(initial_state) atomic → behavior (Initial c) = behavior atomic → atomic = Initial (impl.(initial_state), λ _, Idle).
-  Proof.
-    simpl. intros Hrun. inv Hrun. induction atomic.
-    - intros. inv H2. reflexivity.
-    - intros. inv H2. destruct l; simpl in *.
-      + discriminate.
-      + apply IHatomic in H6; auto. inv H9. simpl in *. inv H2.
-      + discriminate.
-  Qed.
-
-  Lemma complete r atomic σ f : Implementation.Run impl r → Atomic.Run impl.(initial_state) atomic → behavior r = behavior atomic → final atomic = (σ, f) → (final r).(tracker) σ f.
-  Proof.
-    revert atomic σ f.
-    induction r.
-    - simpl. intros. eapply linearization_empty in H2 as ?; eauto. 
-      subst. simpl in *. inv H5. inv H2. simpl. econstructor.
-    - destruct l.
-      + intros. eapply linearization_invoke in H3 as ?; eauto.
-        inv H6 as [atomic' [σ' [f' [πs [? [? [? [? ?]]]]]]]].
-        simpl in *. inv H2. inv H16. simpl. econstructor.
-        * assert (tracker0 = tracker (final r)).
-          { rewrite <- H2. reflexivity. }
-          erewrite H6; eauto.
-        * auto.
-        * eauto.
-      + simpl in *. intros. inv H2. inv H11. simpl. econstructor.
-        * rewrite <- H2 in IHr. simpl in *. eapply IHr; eauto.
-        * econstructor.
-      + intros. eapply linearization_response in H3 as ?; eauto.
-        inv H6 as [atomic' [σ' [f' [πs [? [? [? [? ?]]]]]]]].
-        simpl in *. inv H2. inv H16. simpl.
-        assert (tracker0 = tracker (final r)).
-        { rewrite <- H2. reflexivity. }
-        erewrite H6.
-        econstructor; eauto.
-  Qed.
-
-  (** An implementation is linearizable iff there exists a linearization for each of its runs *)
-  Definition linearizable :=
-    ∀ r,
-      Implementation.Run impl r →
-        ∃ atomic, Atomic.Run impl.(initial_state) atomic ∧ behavior r = behavior atomic.
-
-  Lemma soundness : invariant (λ c, ∃ σ f, tracker c σ f) → linearizable.
-  Proof.
-    unfold linearizable, invariant. intros Hinv r Hrun.
-    pose proof Hinv r Hrun as [σ [f Hmeta]].
-    pose proof sound r Hrun.
-    unfold tracker_sound in *.
-    pose proof H2 _ _ Hmeta as [atomic Hatomic Hlinearization Hfinal].
-    now exists atomic.
-  Qed.
-
-  Lemma completeness : linearizable → invariant (λ c, ∃ σ f, tracker c σ f).
-  Proof.
-    unfold linearizable, invariant. intros Hlinearizable r Hrun.
-    pose proof Hlinearizable r Hrun as [atomic [Hatomic Hbehavior]].
-    destruct (final atomic) as [σ f] eqn:Hfinal.
-    exists σ. exists f.
-    eapply complete; eauto.
-  Qed.
-
-  (* An implementation is linearizable iff its tracker being non-empty is an invariant of the algorithm *)
-  Theorem adequacy : linearizable ↔ invariant (λ c, ∃ σ f, tracker c σ f).
-  Proof.
-    split.
-    - exact completeness.
-    - exact soundness.
-  Qed.
-
-  Lemma partial_full_coupled r r' :
-    Implementation.Run impl r → PartialTracker.Run impl r' → coupled r r' → (final r').(tracker) ⊆ (final r).(tracker).
-  Proof.
-    intros HRun HRunPartial Hcoupled. induction Hcoupled.
-    - reflexivity.
-    - simpl. inv HRun. inv HRunPartial.
-      apply IHHcoupled in H4 as IH; auto. clear H4 H5 IHHcoupled.
-      inv H7; inv H9; (rewrite <- H2 in IH; rewrite <- H3 in IH; simpl in *); etransitivity; eauto.
-      + now apply evolve_inv_monotone.
-      + now apply evolve_monotone.
-      + now apply evolve_ret_monotone.
-  Qed.
-
-End Adequacy.
-
-Section LiftL.
-
-  Context {Π Ω : Type}.
-
-  Context `{Object Π Ω}.
-
-  (* Auxillary objects *)
-  Variable Ω' : Type.
-
-  Context `{Object Π Ω'}.
-
-  (* Definition lift_term_l (e : Term.t Π Ω) :  Term.t Π (Ω + Ω').
-  Proof.
-  Defined. *)
-
-  Fixpoint lift_term_l (e : Term.t Π Ω) : Term.t Π (Ω + Ω') :=
-    match e with
-    | Var x => Var x
-    | Term.Invoke ω op arg => Term.Invoke (inl ω) op (lift_term_l arg)
-    | Bop op e₁ e₂ => Bop op (lift_term_l e₁) (lift_term_l e₂)
-    | Uop op e => Uop op (lift_term_l e)
-    | Term.Pair e₁ e₂ => Term.Pair (lift_term_l e₁) (lift_term_l e₂)
-    | ProjL e => ProjL (lift_term_l e)
-    | ProjR e => ProjR (lift_term_l e)
-    | Term.Int n => Term.Int n
-    | Term.Bool b => Term.Bool b
-    | Term.Unit => Term.Unit
-    end.
-  
-  Local Open Scope dynamics_scope.
-
-  Lemma lift_term_l_complete :
-    ∀ e π ψ (ϵ₁ ϵ₁' : states Π Ω) v (ϵ₂ : states Π Ω'),
-      ⟨ π , arg , ψ , ϵ₁ , e ⟩ ⇓ₑ ⟨ ϵ₁' , v ⟩ →
-        ⟨ π , arg , ψ , disjoint_union ϵ₁ ϵ₂ , lift_term_l e ⟩ ⇓ₑ ⟨ disjoint_union ϵ₁' ϵ₂ , v ⟩.
-  Proof.
-    induction e; intros; simpl in *; inv H1; try (econstructor; eauto).
-    rewrite insert_union_distr_l. econstructor.
-      + eapply IHe. eauto.
-      + inv H8. econstructor. unfold Map.lookup in *. simpl in *. assumption.
-  Qed.
-
-  Lemma lift_term_l_sound_l :
-    ∀ e π ψ ϵ v ϵ',
-      ⟨ π , arg , ψ , ϵ , lift_term_l e ⟩ ⇓ₑ ⟨ ϵ' , v ⟩ →
-        ⟨ π , arg , ψ , πₗ ϵ , e ⟩ ⇓ₑ ⟨ πₗ ϵ' , v ⟩.
-  Proof.
-    induction e; intros; simpl in *; inv H1; try (econstructor; eauto).
-    rewrite πₗ_insert_comm. econstructor.
-    + apply IHe. eassumption.
-    + inv H8. constructor. simpl in *.
-      replace (Map.lookup ω (πₗ ϵ0)) 
-          with (Map.lookup (inl ω) ϵ0) by reflexivity.
-      assumption.
-  Qed.
-
-  Lemma lift_term_l_sound_r :
-    ∀ e π ψ ϵ v ϵ',
-      ⟨ π , arg , ψ , ϵ , lift_term_l e ⟩ ⇓ₑ ⟨ ϵ' , v ⟩ → πᵣ ϵ = πᵣ ϵ'.
-  Proof.
-    induction e; intros; simpl in *; inv H1; intuition.
-    - apply IHe in H7. subst. simpl in *.
-      replace (πᵣ ϵ0) with (πᵣ ϵ'0). apply insert_l_πᵣ.
-    - apply IHe1 in H5. apply IHe2 in H8. congruence.
-    - inv H7. eauto.
-    - apply IHe1 in H4. apply IHe2 in H7. congruence.
-    - apply IHe in H3. assumption.
-    - apply IHe in H3. assumption.
-  Qed.
-
-  Fixpoint lift_stmt_l (s : Stmt.t Π Ω) : Stmt.t Π (Ω + Ω') :=
-    match s with
-    | Seq s₁ s₂ => Seq (lift_stmt_l s₁) (lift_stmt_l s₂)
-    | Assign x e => Assign x (lift_term_l e)
-    | If e s₁ s₂ => If (lift_term_l e) (lift_stmt_l s₁) (lift_stmt_l s₂)
-    | Syntax.Stmt.Goto l => Syntax.Stmt.Goto l
-    | Syntax.Stmt.Return e => Syntax.Stmt.Return (lift_term_l e)
-    | Stmt.Invoke (Invocation ω op arg) => @Syntax.Stmt.Invoke _ (Ω + Ω') _ _ (Invocation (inl ω) op (lift_term_l arg))
-    | Skip => Skip
-    end.
-
-  Lemma lift_stmt_l_complete :
-    ∀ s π ψ ψ' (ϵ₁ ϵ₁' : states Π Ω) sig,
-      ⟨ π , arg , ψ , ϵ₁ , s ⟩ ⇓ₛ ⟨ ψ' , ϵ₁' , sig ⟩ →
-        ∀ ϵ₂,
-          ⟨ π , arg , ψ , disjoint_union ϵ₁ ϵ₂ , lift_stmt_l s ⟩ ⇓ₛ ⟨ ψ' , disjoint_union ϵ₁' ϵ₂ , sig ⟩.
-  Proof.
-    intros. generalize dependent ϵ₂. induction H1; intros.
-    - econstructor.
-    - econstructor. fold lift_stmt_l. eauto.
-    - econstructor. eauto.
-    - econstructor; fold lift_stmt_l; eauto.
-    - econstructor; eauto. eapply lift_term_l_complete. auto.
-    - eapply eval_if_false.
-      + eapply lift_term_l_complete. eauto.
-      + fold lift_stmt_l. eapply IHeval.
-    - econstructor. eapply lift_term_l_complete. eassumption.
-    - econstructor.
-    - econstructor. eapply lift_term_l_complete in H1. eauto.
-    - econstructor. eapply lift_term_l_complete. eassumption.
-  Qed.
-
-  Lemma lift_stmt_l_sound_l :
-    ∀ s π ψ ϵ sig ψ' ϵ',
-      ⟨ π , arg , ψ , ϵ , lift_stmt_l s ⟩ ⇓ₛ ⟨ ψ' , ϵ' , sig ⟩ →
-        ⟨ π , arg , ψ , πₗ ϵ , s ⟩ ⇓ₛ ⟨ ψ' , πₗ ϵ' , sig ⟩.
-  Proof.
-    induction s; intros.
-    - inv H1; econstructor; eauto.
-    - inv H1. econstructor. eapply lift_term_l_sound_l. eassumption.
-    - inv H1.
-      + econstructor.
-        * eapply lift_term_l_sound_l. eassumption.
-        * eauto.
-      + eapply eval_if_false.
-        * eapply lift_term_l_sound_l. eassumption.
-        * eauto.
-    - inv H1. econstructor.
-    - inv H1. econstructor. eapply lift_term_l_sound_l. assumption.
-    - simpl in *. destruct inv. inv H1. econstructor. eapply lift_term_l_sound_l. simpl. eassumption.
-    - inv H1. econstructor.
-  Qed.
-
-  Lemma lift_stmt_l_sound_r :
-    ∀ s π ψ ϵ sig ψ' ϵ',
-      ⟨ π , arg , ψ , ϵ , lift_stmt_l s ⟩ ⇓ₛ ⟨ ψ' , ϵ' , sig ⟩ → πᵣ ϵ = πᵣ ϵ'.
-  Proof.
-    induction s; intros.
-    - inv H1.
-      + eauto.
-      + eauto.
-      + etransitivity.
-        * eapply IHs1. eauto.
-        * eauto.
-    - inv H1. reflexivity.
-    - inv H1.
-      + etransitivity.
-        * eapply lift_term_l_sound_r. eassumption.
-        * eauto.
-      + etransitivity.
-        * eapply lift_term_l_sound_r. eassumption.
-        * eauto.
-    - inv H1. econstructor.
-    - inv H1. eapply lift_term_l_sound_r. eassumption.
-    - cbn in *. destruct inv. inv H1. eapply lift_term_l_sound_r.
-      assert (Term.Invoke (inl ω) op (lift_term_l arg) = lift_term_l (Term.Invoke ω op arg)) by reflexivity.
-      erewrite <- H1.
-      eassumption.
-    - inv H1. econstructor.
-  Qed.
-
-End LiftL.
-
-Section LiftR.
-
-  Context {Π Ω' : Type}.
-
-  Context `{Object Π Ω'}.
-
-  Variable Ω : Type.
-
-  Context `{Object Π Ω}.
-
-  Fixpoint lift_term_r (e : Term.t Π Ω') : Term.t Π (Ω + Ω') :=
-    match e with
-    | Var x => Var x
-    | Term.Invoke ω op arg => @Term.Invoke _ (Ω + Ω') _ _ (inr ω) op (lift_term_r arg)
-    | Bop op e₁ e₂ => Bop op (lift_term_r e₁) (lift_term_r e₂)
-    | Uop op e => Uop op (lift_term_r e)
-    | Term.Pair e₁ e₂ => Term.Pair (lift_term_r e₁) (lift_term_r e₂)
-    | ProjL e => ProjL (lift_term_r e)
-    | ProjR e => ProjR (lift_term_r e)
-    | Term.Int n => Term.Int n
-    | Term.Bool b => Term.Bool b
-    | Term.Unit => Term.Unit
-    end.
-
-  Lemma lift_term_r_complete :
-    ∀ e π ψ (ϵ₂ ϵ₂' : states Π Ω') v (ϵ₁ : states Π Ω),
-      ⟨ π , arg , ψ , ϵ₂ , e ⟩ ⇓ₑ ⟨ ϵ₂' , v ⟩ →
-        ⟨ π , arg , ψ , disjoint_union ϵ₁ ϵ₂ , lift_term_r e ⟩ ⇓ₑ ⟨ disjoint_union ϵ₁ ϵ₂' , v ⟩.
-  Proof.
-    induction e; intros; simpl in *; inv H1; try (econstructor; eauto).
-    rewrite insert_union_distr_r. econstructor.
-      + eapply IHe. eauto.
-      + inv H8. econstructor. unfold Map.lookup in *. simpl in *. assumption.
-  Qed.
-
-  Lemma lift_term_r_sound_r :
-    ∀ e π ψ ϵ v ϵ',
-      ⟨ π , arg , ψ , ϵ , lift_term_r e ⟩ ⇓ₑ ⟨ ϵ' , v ⟩ →
-        ⟨ π , arg , ψ , πᵣ ϵ , e ⟩ ⇓ₑ ⟨ πᵣ ϵ' , v ⟩.
-  Proof.
-    induction e; intros; simpl in *; inv H1; try (econstructor; eauto).
-    rewrite πᵣ_insert_comm. econstructor.
-    + apply IHe. eassumption.
-    + inv H8. constructor. simpl in *.
-      replace (Map.lookup ω (πᵣ ϵ0)) 
-          with (Map.lookup (inr ω) ϵ0) by reflexivity.
-      assumption.
-  Qed.
-
-  Lemma lift_term_r_sound_l :
-    ∀ e π ψ ϵ v ϵ',
-      ⟨ π , arg , ψ , ϵ , lift_term_r e ⟩ ⇓ₑ ⟨ ϵ' , v ⟩ → πₗ ϵ = πₗ ϵ'.
-  Proof.
-    induction e; intros; simpl in *; inv H1; intuition.
-    - apply IHe in H7. simpl in *.
-      replace (πₗ ϵ0) with (πₗ ϵ'0).  apply insert_r_πₗ.
-    - etransitivity.
-      + eapply IHe1. eassumption.
-      + eapply IHe2. eassumption.
-    - inv H7. eauto.
-    - etransitivity.
-      + eapply IHe1. eassumption.
-      + eapply IHe2. eassumption.
-    - eapply IHe. eassumption.
-    - eapply IHe. eassumption.
-  Qed.
-
-  Fixpoint lift_stmt_r (s : Stmt.t Π Ω') : Stmt.t Π (Ω + Ω') :=
-    match s with
-    | Seq s₁ s₂ => Seq (lift_stmt_r s₁) (lift_stmt_r s₂)
-    | Assign x e => Assign x (lift_term_r e)
-    | If e s₁ s₂ => If (lift_term_r e) (lift_stmt_r s₁) (lift_stmt_r s₂)
-    | Syntax.Stmt.Goto l => Syntax.Stmt.Goto l
-    | Syntax.Stmt.Return e => Syntax.Stmt.Return (lift_term_r e)
-    | Stmt.Invoke (Invocation ω op arg) => @Syntax.Stmt.Invoke _ (Ω + Ω') _ _ (@Invocation _ (Ω + Ω') _ _ (inr ω) op (lift_term_r arg))
-    | Skip => Skip
-    end.
-
-  Lemma lift_stmt_r_complete :
-    ∀ s π ψ ψ' (ϵ₂ ϵ₂' : states Π Ω') sig,
-      ⟨ π , arg , ψ , ϵ₂ , s ⟩ ⇓ₛ ⟨ ψ' , ϵ₂' , sig ⟩ →
-        ∀ ϵ₁,
-          ⟨ π , arg , ψ , disjoint_union ϵ₁ ϵ₂ , lift_stmt_r s ⟩ ⇓ₛ ⟨ ψ' , disjoint_union ϵ₁ ϵ₂' , sig ⟩.
-  Proof.
-    intros. generalize dependent ϵ₁. induction H1; intros.
-    - econstructor.
-    - econstructor. fold lift_stmt_r. eauto.
-    - econstructor. eauto.
-    - econstructor; fold lift_stmt_r; eauto.
-    - econstructor; eauto. eapply lift_term_r_complete. auto.
-    - eapply eval_if_false.
-      + eapply lift_term_r_complete. eauto.
-      + fold lift_stmt_r. eapply IHeval.
-    - econstructor. eapply lift_term_r_complete. eassumption.
-    - econstructor.
-    - econstructor. eapply lift_term_r_complete in H1. eauto.
-    - econstructor. eapply lift_term_r_complete. eassumption.
-  Qed.
-
-  Lemma lift_stmt_r_sound_r :
-    ∀ s π ψ ϵ sig ψ' ϵ',
-      ⟨ π , arg , ψ , ϵ , lift_stmt_r s ⟩ ⇓ₛ ⟨ ψ' , ϵ' , sig ⟩ →
-        ⟨ π , arg , ψ , πᵣ ϵ , s ⟩ ⇓ₛ ⟨ ψ' , πᵣ ϵ' , sig ⟩.
-  Proof.
-    induction s; intros.
-    - inv H1; econstructor; eauto.
-    - inv H1. econstructor. eapply lift_term_r_sound_r. eassumption.
-    - inv H1.
-      + econstructor.
-        * eapply lift_term_r_sound_r. eassumption.
-        * eauto.
-      + eapply eval_if_false.
-        * eapply lift_term_r_sound_r. eassumption.
-        * eauto.
-    - inv H1. econstructor.
-    - inv H1. econstructor. eapply lift_term_r_sound_r. assumption.
-    - simpl in *. destruct inv. inv H1. econstructor. eapply lift_term_r_sound_r. simpl. eassumption.
-    - inv H1. econstructor.
-  Qed.
-
-  Lemma lift_stmt_r_sound_l :
-    ∀ s π ψ ϵ sig ψ' ϵ',
-      ⟨ π , arg , ψ , ϵ , lift_stmt_r s ⟩ ⇓ₛ ⟨ ψ' , ϵ' , sig ⟩ → πₗ ϵ = πₗ ϵ'.
-  Proof.
-    induction s; intros.
-    - inv H1.
-      + eauto.
-      + eauto.
-      + etransitivity.
-        * eapply IHs1. eauto.
-        * eauto.
-    - inv H1. reflexivity.
-    - inv H1.
-      + etransitivity.
-        * eapply lift_term_r_sound_l. eassumption.
-        * eauto.
-      + etransitivity.
-        * eapply lift_term_r_sound_l. eassumption.
-        * eauto.
-    - inv H1. econstructor.
-    - inv H1. eapply lift_term_r_sound_l. eassumption.
-    - cbn in *. destruct inv. inv H1. eapply lift_term_r_sound_l.
-      assert (@Term.Invoke _ (Ω + Ω') _ _ (inr _) op (lift_term_r arg) = lift_term_r (Term.Invoke ω op arg)) by reflexivity.
-      erewrite <- H1.
-      eassumption.
-    - inv H1. econstructor.
-  Qed.
-
-End LiftR.
